ECCA renamings, but not yet renamed in translation files. reorganizing

ECCA/continuations.v
@@ -1,5 +1,5 @@
-Require Export ECCA_typing.
-Require Import ECCA_core_lemmas.
+Require Export typing.
+Require Import core_lemmas.
 
 (*===========================
   ==--Continuation Typing--==
@@ -9,14 +9,14 @@ Require Import ECCA_core_lemmas.
 
 Inductive cont {V: nat}: Type :=
   | Hole
-  | LetHole (B: @ECCAexp (S V))
+  | LetHole (B: @exp (S V))
 .
 Hint Constructors cont.
 Bind Scope ECCA_scope with cont.
 
 Inductive cont_r {V: nat}: Type :=
   | rHole
-  | rLetHole (B: @ECCAconf (S V))
+  | rLetHole (B: @conf (S V))
 .
 Hint Constructors cont_r.
 Bind Scope ECCA_scope with cont_r.
@@ -24,17 +24,17 @@ Bind Scope ECCA_scope with cont_r.
 Fixpoint unrestrict_cont {V: nat}(k: @cont_r V): @cont V:=
 match k with
   | rHole => Hole
-  | rLetHole B => LetHole (flattenECCAconf B)
+  | rLetHole B => LetHole (flattenconf B)
 end.
 
-Definition fill_hole {V: nat}(e: @ECCAexp V) (K: @cont V): @ECCAexp V:=
+Definition fill_hole {V: nat}(e: @exp V) (K: @cont V): @exp V:=
   match K with
     | Hole => e
     | LetHole B => eLet e B
 end.
 Notation "K '[' N ']'" := (fill_hole N K) (at level 200): ECCA_scope.
 
-Definition fill_hole_r {V: nat}(e: @ECCAcomp V) (K: @cont_r V): @ECCAconf V:=
+Definition fill_hole_r {V: nat}(e: @comp V) (K: @cont_r V): @conf V:=
   match K with
     | rHole => e
     | rLetHole B => Let e B
@@ -42,29 +42,29 @@ end.
 
 Notation "'[]'" := (Hole) (at level 50) : ECCA_scope.
 Notation "'LET' '_' ':=' '[]' 'in' B" := (LetHole B) (at level 50) : ECCA_scope.
-Definition exId: @ECCAexp 1 := (eId (@bound 1 l0)).
+Definition exId: @exp 1 := (eId (@bound 1 l0)).
 Definition example_aLetHole := (LET _ := [] in (eId (@bound 1 l0)))%ECCA.
 Definition ex_fillhole := (fill_hole (eTru) example_aLetHole).
 
 Inductive cont_type {V: nat}: Type :=
-  | Cont (M: @ECCAexp V) (A: @ECCAexp V) (B: @ECCAexp V)
+  | Cont (M: @exp V) (A: @exp V) (B: @exp V)
 .
 Hint Constructors cont_type.
 (* TODO: Add notation for cont type  *)
 
-Inductive ECCA_cont_has_type : ECCAenv -> cont  -> cont_type -> Prop :=
-  | aK_Empty (M: ECCAexp) (g: ECCAenv) (A: ECCAexp):
-    ECCA_has_type g M A ->
-    ECCA_cont_has_type g Hole (Cont M A A)
-  | aK_Bind (g: ECCAenv) (y: name) (M: ECCAexp) (M' A B: @ECCAexp 0):
-    ECCA_has_type g M' A ->
-    ECCA_has_type (ctx_cons g y (Def M' A)) (open y M) (open y (wk B)) ->
-    ECCA_cont_has_type g (LetHole M) (Cont M' A B)
+Inductive Types_cont : env -> cont  -> cont_type -> Prop :=
+  | aK_Empty (M: exp) (g: env) (A: exp):
+    Types g M A ->
+    Types_cont g Hole (Cont M A A)
+  | aK_Bind (g: env) (y: name) (M: exp) (M' A B: @exp 0):
+    Types g M' A ->
+    Types (ctx_cons g y (Def M' A)) (open y M) (open y (wk B)) ->
+    Types_cont g (LetHole M) (Cont M' A B)
 .
 
-Hint Constructors ECCA_cont_has_type.
+Hint Constructors Types_cont.
 
-Lemma fill_with_hole_is_id {V: nat}(e: @ECCAexp V): fill_hole e Hole = e.
+Lemma fill_with_hole_is_id {V: nat}(e: @exp V): fill_hole e Hole = e.
 Proof.
 eauto. Qed.
 
