ECCA/core_lemmas.v
@@ -1,0 +1,776 @@
+Require Import core.
+
+(* How do we unbox this result given that we have proven it is never None? Three ways!*)
+
+
+(* Definition unoption_neq {T: Type}(e: option T) : e <> None -> T.
+Proof.
+intros. destruct e.
+exact t.
+contradiction.
+Defined.
+
+thanks to pgiarrusso in freenode/#coq
+
+Definition unoption_sig {T: Type}(o: option T): {n: T | o = Some n } -> T.
+Proof. intros.
+destruct X. exact x.
+Defined. *)
+
+Definition unoption_ex {T: Type}(o : option T) : (exists (n : T), o = Some n) -> T.
+Proof. intros.
+destruct o.
+exact t.
+exfalso. destruct H. discriminate.
+Defined.
+
+
+Definition invertsval {V: nat} (e: @val V) :=
+getval (flattenval e) = Some e.
+Definition invertsconf {V: nat} (e: @conf V) :=
+getconf (flattenconf e) = Some e.
+Definition invertscomp {V: nat} (e: @comp V) :=
+getcomp (flattencomp e) = Some e.
+
+Lemma helper_val {V: nat}:
+forall (v1: @val V),
+match getconf (flattenval v1) with
+    | Some (Comp (Val e)) => Some e
+    | _ => None
+    end = Some v1 
+-> getconf(flattenval v1) = Some (Comp (Val v1)).
+Proof. intros. destruct (getconf (flattenval v1)); try discriminate.
+destruct c; try discriminate. destruct e; try discriminate. inversion H. reflexivity.
+Defined.
+
+(* TODO: should write an LTAC tactic that does this: simplifies equalities involving match *)
+(* Ltac simplmatcheq:=
+  (* repeat *) match goal with 
+  | [ H:  match ?x with  
+      | _ => ?b
+      | _ => ?c
+    end = ?v |- _ ] => idtac "hello"
+  end. *)
+Lemma helper_comp {V: nat}:
+forall (v1: @comp V),
+match getconf (flattencomp v1) with
+    | Some (Comp e) => Some e
+    | _ => None
+    end = Some v1 
+-> getconf(flattencomp v1) = Some (Comp v1).
+Proof. intros. destruct (getconf (flattencomp v1)); try discriminate.
+destruct c; try discriminate. destruct e; try discriminate; inversion H; reflexivity.
+Defined.
+
+Lemma get_inverts_flatten {V: nat}: 
+   (forall (e: @val V), invertsval e) 
+/\ (forall (e: @conf V), invertsconf e)
+/\ (forall (e: @comp V), invertscomp e).
+Proof. apply val_conf_comp_comb.
+1,2,7,8,9: (intros; cbv; auto).
+1,2,3: intros; unfold invertsval, invertsconf in *; cbn; unfold getval. 
++ cut (getconf (ePi (flattenconf A) (flattenconf B)) = Some (Comp (Val (Pi A B)))).
+ - intros. rewrite H1. auto.
+ - cbn. rewrite H. rewrite H0. auto.
++ cut (getconf (eAbs (flattenconf A) (flattenconf B)) = Some (Comp (Val (Abs A B)))).
+ - intros. rewrite H1. auto.
+ - cbn. rewrite H. rewrite H0. auto.
++ cut (getconf (eSig (flattenconf A) (flattenconf B)) = Some (Comp (Val (Sig A B)))).
+ - intros. rewrite H1. auto.
+ - cbn. rewrite H. rewrite H0. auto.
++ intros; unfold invertsval, invertsconf in *. 
+   apply helper_val in H. apply helper_val in H0.
+   unfold getval. cbn. rewrite H. rewrite H0.
+   rewrite H1. auto.
++ intros. unfold invertscomp, invertsconf in *. apply helper_comp in H.
+  cbn. auto.
++ intros. unfold invertscomp, invertsconf in *. apply helper_comp in H.
+  cbn. rewrite H. rewrite H0. auto.
++ intros. unfold invertsconf, invertsval, invertscomp in *. cbn.
+  apply helper_val in H. rewrite H. rewrite H0. rewrite H1. auto.
++ intros. unfold invertscomp, invertsval in *. apply helper_val in H.
+  apply helper_val in H0. unfold getcomp.
+  cbn. rewrite H. rewrite H0. auto.
++ intros; unfold invertscomp, invertsval in *; apply helper_val in H;
+  unfold getcomp; cbn; rewrite H; auto.
++ intros; unfold invertscomp, invertsval in *; apply helper_val in H;
+  unfold getcomp; cbn; rewrite H; auto.
++ intros; unfold invertscomp, invertsval in *; apply helper_val in H;
+  unfold getcomp; cbn; rewrite H; auto.
+Defined.
+
+Definition reflectsval {V: nat} (e: @val V):=
+isVal (flattenval e).
+Definition reflectsconf {V: nat} (e: @conf V):=
+isConf (flattenconf e).
+Definition reflectscomp {V: nat} (e: @comp V):=
+isComp (flattencomp e).
+
+Lemma flatten_is_ANF {V: nat}:
+   (forall (e: @val V), reflectsval e) 
+/\ (forall (e: @conf V), reflectsconf e)
+/\ (forall (e: @comp V), reflectscomp e).
+Proof. repeat split. all: intros; exists e; apply get_inverts_flatten.
+Defined.
+
+Corollary flatten_conf_is_ANF {V: nat}:
+(forall (e: @conf V), isConf (flattenconf e)).
+Proof. apply flatten_is_ANF. Defined.
+
+Corollary flatten_val_is_ANF {V: nat}:
+(forall (e: @val V), isVal (flattenval e)).
+Proof. apply flatten_is_ANF. Defined.
+
+Corollary flatten_comp_is_ANF {V: nat}:
+(forall (e: @comp V), isComp (flattencomp e)).
+Proof. apply flatten_is_ANF. Defined.
+
+Lemma wk_preserves_ANF {V: nat}:
+forall (e: @exp V), 
+(isVal e -> isVal (wk e))
+/\ (isConf e -> isConf (wk e)) 
+/\ (isComp e -> isComp (wk e)).
+Proof. induction e.
++ repeat split.
+  - intros.
+    cbn. unfold isVal. exists (Id (wkv x)). auto.
+  - intros. unfold isConf.
+    cbn. exists (Comp (Val (Id (wkv x)))). auto.
+  - intros.
+    unfold isComp. cbn.
+    exists (Val (Id (wkv x))). auto.
++ repeat split; cbv; eauto.
++ intros. unfold isConf, isVal, isComp in *. 
+  try destruct IHe1, IHe2.
+  destruct H0, H2.
+  repeat split; intros.
+  1: unfold getval; unfold getval in H5.
+  3: unfold getcomp; unfold getcomp in H5. 
+  all:  destruct H5; cbn in H5;
+    destruct getconf eqn:Heq1 in H5; try discriminate;
+    destruct getconf eqn:Heq2 in H5; try discriminate;
+    cbn; destruct H0; eauto; destruct H2; eauto;
+    cbn in H0, H2; rewrite H0, H2;
+    eauto.
++ intros. unfold isConf, isVal, isComp in *. 
+  try destruct IHe1, IHe2.
+  destruct H0, H2.
+  repeat split; intros.
+  1: unfold getval; unfold getval in H5.
+  3: unfold getcomp; unfold getcomp in H5. 
+  all:  destruct H5; cbn in H5;
+    destruct getconf eqn:Heq1 in H5; try discriminate;
+    destruct getconf eqn:Heq2 in H5; try discriminate;
+    cbn; destruct H0; eauto; destruct H2; eauto;
+    cbn in H0, H2; rewrite H0, H2;
+    eauto.
++ intros. unfold isConf, isVal, isComp in *. 
+  try destruct IHe1, IHe2.
+  destruct H0, H2.
+  repeat split; intros.
+  1: unfold getval; unfold getval in H5.
+  3: unfold getcomp; unfold getcomp in H5. 
+  all:  destruct H5; cbn in H5;
+    destruct getconf eqn:Heq1 in H5; try discriminate;
+    destruct getconf eqn:Heq2 in H5; try discriminate;
+    cbn; destruct H0; eauto; destruct H2; eauto;
+    cbn in H0, H2; rewrite H0, H2;
+    eauto.
++ intros. unfold isConf, isVal, isComp in *. 
+  try destruct IHe1, IHe2, IHe3.
+  destruct H0, H2, H4.
+  repeat split; intros.
+  1: unfold getval in H8.
+  3: unfold getcomp in H8.
+  all:
+    cbn in H8; destruct H8; 
+    destruct getconf eqn:? in H8; try discriminate;
+    destruct c eqn:? in H8; try discriminate;
+    destruct e eqn:? in H8; try discriminate;
+    subst;
+    destruct getconf eqn:? in H8; try discriminate;
+    destruct c eqn:? in H8; try discriminate;
+    destruct e eqn:? in H8; try discriminate;
+    subst;
+    destruct getconf eqn:? in H8; try discriminate.
+  1: unfold getval. 
+  3: unfold getcomp. 
+  all:
+    cbn;
+    unfold getval in H; destruct H; try rewrite Heqo; eauto;
+    destruct getconf eqn:? in H ; try discriminate;
+    destruct c0 eqn:? in H ; try discriminate;
+    destruct e eqn:? in H ; try discriminate;
+    subst; cbn in Heqo2; rewrite Heqo2;
+
+    unfold getval in H1; destruct H1; try rewrite Heqo0; eauto;
+    destruct getconf eqn:? in H1; try discriminate;
+    destruct c0 eqn:? in H1; try discriminate;
+    destruct e eqn:? in H1; try discriminate;
+    subst; cbn in Heqo3; rewrite Heqo3;
+
+    destruct H4; eauto; cbn in H4; rewrite H4; eauto.
++ repeat split; intros; cbn; (unfold isVal || unfold isConf || unfold isComp); cbn; eauto.
++ repeat split; intros; cbn; (unfold isVal || unfold isConf || unfold isComp); cbn; eauto.
++ repeat split; intros; cbn; (unfold isVal || unfold isConf || unfold isComp); cbn; eauto.
++ repeat split; intros; 
+  destruct IHe1, IHe2; 
+  destruct H1, H3;
+  unfold isConf, isVal, isComp in *. 
+  - unfold isVal; unfold getval; cbn. 
+    destruct H. unfold getval in H. cbn in H.
+    destruct getconf eqn:? in H; try discriminate.
+    destruct c eqn:? in H; try discriminate.
+    destruct getconf eqn:? in H; try discriminate.
+  - cbn. 
+    destruct H. cbn in H.
+    destruct getconf eqn:? in H; try discriminate.
+    destruct c eqn:? in H; try discriminate.
+    subst.
+    destruct getconf eqn:? in H; try discriminate.
+   
+    unfold getcomp in H4. rewrite Heqo in H4. 
+    destruct H4; eauto. 
+    destruct getconf eqn:? in H4; try discriminate.
+    destruct c0 eqn:? in H4; try discriminate. subst.
+    cbn in Heqo1. rewrite Heqo1.
+
+    rewrite Heqo0 in H3. destruct H3; eauto.
+    cbn in H3. rewrite H3. eauto.
+  - unfold isComp; unfold getcomp; cbn. 
+    destruct H. unfold getcomp in H. cbn in H.
+    destruct getconf eqn:? in H; try discriminate.
+    destruct c eqn:? in H; try discriminate.
+    destruct getconf eqn:? in H; try discriminate.
++ repeat split; intros; destruct IHe1, IHe2, IHe3; destruct H1, H3, H5;
+    unfold isConf, isVal, isComp in *. 
+  1: unfold getval; unfold getval in H.
+  3: unfold getcomp; unfold getcomp in H.
+  all: cbn.
+  all:  destruct H; unfold getval in H; cbn in H;
+    destruct getconf eqn:? in H; try discriminate;
+    destruct getconf eqn:? in H; try discriminate;
+    destruct getconf eqn:? in H; try discriminate;
+    destruct c1 eqn:? in H; try discriminate;
+    destruct e eqn:? in H; try discriminate.
+  - subst.
+    rewrite Heqo in H3. destruct H3; eauto.
+    cbn in H3. rewrite H3.
+    rewrite Heqo0 in H5. destruct H5; eauto.
+    cbn in H5. rewrite H5.
+    unfold getval in H0. rewrite Heqo1 in H0. destruct H0; eauto.
+    destruct getconf eqn:? in H0; try discriminate. 
+    destruct c1 eqn:? in H0; try discriminate.
+    destruct e eqn:? in H0; try discriminate.
+    subst.
+    cbn in Heqo2. rewrite Heqo2. eauto.
++ repeat split; intros; destruct IHe1, IHe2; destruct H1, H3;
+  unfold isConf, isVal, isComp in *.
+  3: unfold getcomp in H; unfold getcomp.
+  1: unfold getval in H.
+  all: destruct H; cbn in H;
+    destruct getconf eqn:? in H; try discriminate;
+    destruct c eqn:? in H; try discriminate;
+    destruct e eqn:? in H; try discriminate;
+    subst;
+    destruct getconf eqn:? in H; try discriminate;
+    destruct c eqn:? in H; try discriminate;
+    destruct e eqn:? in H; try discriminate.
+  all:
+    subst; cbn;
+    unfold getval in H0; rewrite Heqo in H0;  destruct H0; eauto; 
+    destruct getconf eqn:? in H0; try discriminate; 
+    destruct c eqn:? in H0; try discriminate;
+    destruct e eqn:? in H0; try discriminate; subst;
+    cbn in Heqo1; rewrite Heqo1;
+    unfold getval in H2; rewrite Heqo0 in H2;  destruct H2; eauto; 
+    destruct getconf eqn:? in H2; try discriminate; 
+    destruct c eqn:? in H2; try discriminate;
+    destruct e eqn:? in H2; try discriminate; subst;
+    cbn in Heqo2; rewrite Heqo2; eauto.
++ repeat split; intros; destruct IHe; destruct H1;
+  unfold isConf, isVal, isComp in *.
+  1: unfold getval in H; unfold getval.
+  3: unfold getcomp in H; unfold getcomp.
+  all: cbn in H; destruct H; 
+    destruct getconf eqn:? in H; try discriminate;
+    destruct c eqn:? in H; try discriminate;
+    destruct e0 eqn:? in H; try discriminate.
+  all: subst; cbn; unfold getval in H0; rewrite Heqo in H0; destruct H0; eauto;
+    destruct getconf eqn:? in H0; try discriminate;
+    destruct c eqn:? in H0; try discriminate;
+    destruct e0 eqn:? in H0; try discriminate;
+    subst; cbn in Heqo0; rewrite Heqo0; eauto.
++ repeat split; intros; destruct IHe; destruct H1;
+  unfold isConf, isVal, isComp in *.
+  1: unfold getval in H; unfold getval.
+  3: unfold getcomp in H; unfold getcomp.
+  all: cbn in H; destruct H; 
+    destruct getconf eqn:? in H; try discriminate;
+    destruct c eqn:? in H; try discriminate;
+    destruct e0 eqn:? in H; try discriminate.
+  all: subst; cbn; unfold getval in H0; rewrite Heqo in H0; destruct H0; eauto;
+    destruct getconf eqn:? in H0; try discriminate;
+    destruct c eqn:? in H0; try discriminate;
+    destruct e0 eqn:? in H0; try discriminate;
+    subst; cbn in Heqo0; rewrite Heqo0; eauto.
+Defined.
+
+Corollary wk_preserves_conf {V: nat}: 
+forall (e: @exp V), (isConf e -> isConf (wk e)).
+Proof. apply wk_preserves_ANF. Defined.
+
+Corollary wk_preserves_val {V: nat}: 
+forall (e: @exp V), (isVal e -> isVal (wk e)).
+Proof. apply wk_preserves_ANF. Defined.
+
+Corollary wk_preserves_comp {V: nat}: 
+forall (e: @exp V), (isComp e -> isComp (wk e)).
+Proof. apply wk_preserves_ANF. Defined.
+
+Compute (unoption_ex (getval (wk (flattenval (Tru))))) ((wk_preserves_val (flattenval (Tru))) (flatten_val_is_ANF Tru)).
+Definition wk_val {V: nat}(e: @val V) :=
+(unoption_ex (getval (wk (flattenval (e))))) ((wk_preserves_val (flattenval e)) (flatten_val_is_ANF e)).
+Definition wk_comp {V: nat}(e: @comp V):=
+(unoption_ex (getcomp (wk (flattencomp (e))))) ((wk_preserves_comp (flattencomp e)) (flatten_comp_is_ANF e)).
+Definition wk_conf {V: nat}(e: @conf V):=
+(unoption_ex (getconf (wk (flattenconf (e))))) ((wk_preserves_conf (flattenconf e)) (flatten_conf_is_ANF e)).
+
+Lemma close_preserves_ANF {V: nat} (x: name):
+forall (e: @exp V), 
+(isVal e -> isVal (close x e))
+/\ (isConf e -> isConf (close x e)) 
+/\ (isComp e -> isComp (close x e)).
+Proof. induction e.
++ repeat split.
+  - intros.
+    cbn. unfold isVal. exists (Id (closev x x0)). auto.
+  - intros. unfold isConf.
+    cbn. exists (Comp (Val (Id (closev x x0)))). auto.
+  - intros.
+    unfold isComp. cbn.
+    exists (Val (Id (closev x x0))). auto.
++ repeat split; cbv; eauto.
++ intros. unfold isConf, isVal, isComp in *. 
+  try destruct IHe1, IHe2.
+  destruct H0, H2.
+  repeat split; intros.
+  1: unfold getval; unfold getval in H5.
+  3: unfold getcomp; unfold getcomp in H5. 
+  all:  destruct H5; cbn in H5;
+    destruct getconf eqn:Heq1 in H5; try discriminate;
+    destruct getconf eqn:Heq2 in H5; try discriminate;
+    cbn; destruct H0; eauto; destruct H2; eauto;
+    cbn in H0, H2; rewrite H0, H2;
+    eauto.
++ intros. unfold isConf, isVal, isComp in *. 
+  try destruct IHe1, IHe2.
+  destruct H0, H2.
+  repeat split; intros.
+  1: unfold getval; unfold getval in H5.
+  3: unfold getcomp; unfold getcomp in H5. 
+  all:  destruct H5; cbn in H5;
+    destruct getconf eqn:Heq1 in H5; try discriminate;
+    destruct getconf eqn:Heq2 in H5; try discriminate;
+    cbn; destruct H0; eauto; destruct H2; eauto;
+    cbn in H0, H2; rewrite H0, H2;
+    eauto.
++ intros. unfold isConf, isVal, isComp in *. 
+  try destruct IHe1, IHe2.
+  destruct H0, H2.
+  repeat split; intros.
+  1: unfold getval; unfold getval in H5.
+  3: unfold getcomp; unfold getcomp in H5. 
+  all:  destruct H5; cbn in H5;
+    destruct getconf eqn:Heq1 in H5; try discriminate;
+    destruct getconf eqn:Heq2 in H5; try discriminate;
+    cbn; destruct H0; eauto; destruct H2; eauto;
+    cbn in H0, H2; rewrite H0, H2;
+    eauto.
++ intros. unfold isConf, isVal, isComp in *. 
+  try destruct IHe1, IHe2, IHe3.
+  destruct H0, H2, H4.
+  repeat split; intros.
+  1: unfold getval in H8.
+  3: unfold getcomp in H8.
+  all:
+    cbn in H8; destruct H8; 
+    destruct getconf eqn:? in H8; try discriminate;
+    destruct c eqn:? in H8; try discriminate;
+    destruct e eqn:? in H8; try discriminate;
+    subst;
+    destruct getconf eqn:? in H8; try discriminate;
+    destruct c eqn:? in H8; try discriminate;
+    destruct e eqn:? in H8; try discriminate;
+    subst;
+    destruct getconf eqn:? in H8; try discriminate.
+  1: unfold getval. 
+  3: unfold getcomp.
+  all:
+    cbn;
+    unfold getval in H; destruct H; try rewrite Heqo; eauto;
+    destruct getconf eqn:? in H ; try discriminate;
+    destruct c0 eqn:? in H ; try discriminate;
+    destruct e eqn:? in H ; try discriminate;
+    subst; cbn in Heqo2; rewrite Heqo2;
+
+    unfold getval in H1; destruct H1; try rewrite Heqo0; eauto;
+    destruct getconf eqn:? in H1; try discriminate;
+    destruct c0 eqn:? in H1; try discriminate;
+    destruct e eqn:? in H1; try discriminate;
+    subst; cbn in Heqo3; rewrite Heqo3;
+
+    destruct H4; eauto; cbn in H4; rewrite H4; eauto.
++ repeat split; intros; cbn; (unfold isVal || unfold isConf || unfold isComp); cbn; eauto.
++ repeat split; intros; cbn; (unfold isVal || unfold isConf || unfold isComp); cbn; eauto.
++ repeat split; intros; cbn; (unfold isVal || unfold isConf || unfold isComp); cbn; eauto.
++ repeat split; intros; 
+  destruct IHe1, IHe2; 
+  destruct H1, H3;
+  unfold isConf, isVal, isComp in *. 
+  - unfold isVal; unfold getval; cbn. 
+    destruct H. unfold getval in H. cbn in H.
+    destruct getconf eqn:? in H; try discriminate.
+    destruct c eqn:? in H; try discriminate.
+    destruct getconf eqn:? in H; try discriminate.
+  - cbn. 
+    destruct H. cbn in H.
+    destruct getconf eqn:? in H; try discriminate.
+    destruct c eqn:? in H; try discriminate.
+    subst.
+    destruct getconf eqn:? in H; try discriminate.
+   
+    unfold getcomp in H4. rewrite Heqo in H4. 
+    destruct H4; eauto. 
+    destruct getconf eqn:? in H4; try discriminate.
+    destruct c0 eqn:? in H4; try discriminate. subst.
+    cbn in Heqo1. rewrite Heqo1.
+
+    rewrite Heqo0 in H3. destruct H3; eauto.
+    cbn in H3. rewrite H3. eauto.
+  - unfold isComp; unfold getcomp; cbn. 
+    destruct H. unfold getcomp in H. cbn in H.
+    destruct getconf eqn:? in H; try discriminate.
+    destruct c eqn:? in H; try discriminate.
+    destruct getconf eqn:? in H; try discriminate.
++ repeat split; intros; destruct IHe1, IHe2, IHe3; destruct H1, H3, H5;
+    unfold isConf, isVal, isComp in *. 
+  1: unfold getval; unfold getval in H.
+  3: unfold getcomp; unfold getcomp in H.
+  all: cbn.
+  all:  destruct H; unfold getval in H; cbn in H;
+    destruct getconf eqn:? in H; try discriminate;
+    destruct getconf eqn:? in H; try discriminate;
+    destruct getconf eqn:? in H; try discriminate;
+    destruct c1 eqn:? in H; try discriminate;
+    destruct e eqn:? in H; try discriminate.
+  - subst.
+    rewrite Heqo in H3. destruct H3; eauto.
+    cbn in H3. rewrite H3.
+    rewrite Heqo0 in H5. destruct H5; eauto.
+    cbn in H5. rewrite H5.
+    unfold getval in H0. rewrite Heqo1 in H0. destruct H0; eauto;
+    destruct getconf eqn:? in H0; try discriminate;
+    destruct c1 eqn:? in H0; try discriminate;
+    destruct e eqn:? in H0; try discriminate.
+    subst.
+    cbn in Heqo2. rewrite Heqo2. eauto.
++ repeat split; intros; destruct IHe1, IHe2; destruct H1, H3;
+  unfold isConf, isVal, isComp in *.
+  3: unfold getcomp in H; unfold getcomp.
+  1: unfold getval in H.
+  all: destruct H; cbn in H;
+    destruct getconf eqn:? in H; try discriminate;
+    destruct c eqn:? in H; try discriminate;
+    destruct e eqn:? in H; try discriminate;
+    subst;
+    destruct getconf eqn:? in H; try discriminate;
+    destruct c eqn:? in H; try discriminate;
+    destruct e eqn:? in H; try discriminate.
+  all:
+    subst; cbn;
+    unfold getval in H0; rewrite Heqo in H0;  destruct H0; eauto; 
+    destruct getconf eqn:? in H0; try discriminate; 
+    destruct c eqn:? in H0; try discriminate;
+    destruct e eqn:? in H0; try discriminate; subst;
+    cbn in Heqo1; rewrite Heqo1;
+    unfold getval in H2; rewrite Heqo0 in H2;  destruct H2; eauto; 
+    destruct getconf eqn:? in H2; try discriminate; 
+    destruct c eqn:? in H2; try discriminate;
+    destruct e eqn:? in H2; try discriminate; subst;
+    cbn in Heqo2; rewrite Heqo2; eauto.
++ repeat split; intros; destruct IHe; destruct H1;
+  unfold isConf, isVal, isComp in *.
+  1: unfold getval in H; unfold getval.
+  3: unfold getcomp in H; unfold getcomp.
+  all: cbn in H; destruct H; 
+    destruct getconf eqn:? in H; try discriminate;
+    destruct c eqn:? in H; try discriminate;
+    destruct e0 eqn:? in H; try discriminate.
+  all: subst; cbn; unfold getval in H0; rewrite Heqo in H0; destruct H0; eauto;
+    destruct getconf eqn:? in H0; try discriminate;
+    destruct c eqn:? in H0; try discriminate;
+    destruct e0 eqn:? in H0; try discriminate;
+    subst; cbn in Heqo0; rewrite Heqo0; eauto.
++ repeat split; intros; destruct IHe; destruct H1;
+  unfold isConf, isVal, isComp in *.
+  1: unfold getval in H; unfold getval.
+  3: unfold getcomp in H; unfold getcomp.
+  all: cbn in H; destruct H; 
+    destruct getconf eqn:? in H; try discriminate;
+    destruct c eqn:? in H; try discriminate;
+    destruct e0 eqn:? in H; try discriminate.
+  all: subst; cbn; unfold getval in H0; rewrite Heqo in H0; destruct H0; eauto;
+    destruct getconf eqn:? in H0; try discriminate;
+    destruct c eqn:? in H0; try discriminate;
+    destruct e0 eqn:? in H0; try discriminate;
+    subst; cbn in Heqo0; rewrite Heqo0; eauto.
+Defined.
+
+Corollary close_preserves_conf {V: nat} (x: name): 
+forall (e: @exp V), (isConf e -> isConf (close x e)).
+Proof. apply close_preserves_ANF. Defined.
+
+Corollary close_preserves_val {V: nat} (x: name): 
+forall (e: @exp V), (isVal e -> isVal (close x e)).
+Proof. apply close_preserves_ANF. Defined.
+
+Corollary close_preserves_comp {V: nat} (x: name): 
+forall (e: @exp V), (isComp e -> isComp (close x e)).
+Proof. apply close_preserves_ANF. Defined.
+
+Definition close_val {V: nat}(x: name)(e: @val V) :=
+(unoption_ex (getval (close x (flattenval (e))))) ((close_preserves_val x (flattenval e)) (flatten_val_is_ANF e)).
+Definition close_comp {V: nat}(x: name)(e: @comp V):=
+(unoption_ex (getcomp (close x (flattencomp (e))))) ((close_preserves_comp x (flattencomp e)) (flatten_comp_is_ANF e)).
+Definition close_conf {V: nat}(x: name)(e: @conf V):=
+(unoption_ex (getconf (close x (flattenconf (e))))) ((close_preserves_conf x (flattenconf e)) (flatten_conf_is_ANF e)).
+
+
+Require Import Coq.Program.Equality.
+
+Lemma open_preserves_ANF {V: nat} (x: name):
+forall (e: @exp (S V)), 
+(@isVal (S V) e -> @isVal V (open x e))
+/\ (@isConf (S V) e -> @isConf V (open x e)) 
+/\ (@isComp (S V) e -> @isComp V (open x e)).
+Proof. dependent induction e.
++ repeat split.
+  - intros.
+    cbn. unfold isVal. exists (Id (openv x x0)). auto.
+  - intros. unfold isConf.
+    cbn. exists (Comp (Val (Id (openv x x0)))). auto.
+  - intros.
+    unfold isComp. cbn.
+    exists (Val (Id (openv x x0))). auto.
++ repeat split; cbv; eauto.
++ intros. unfold isConf, isVal, isComp in *.
+  destruct IHe1 with (V0:=V) (e0 := e1); auto.
+  destruct IHe2  with (V0:=S V) (e0 := e2); auto.
+  destruct H0, H2.
+  repeat split; intros.
+  1: unfold getval; unfold getval in H5.
+  3: unfold getcomp; unfold getcomp in H5. 
+  all: destruct H5; cbn in H5;
+    destruct getconf eqn:Heq1 in H5; try discriminate;
+    destruct getconf eqn:Heq2 in H5; try discriminate;
+    cbn; destruct H0; eauto; destruct H2; eauto;
+    cbn in H0, H2; rewrite H0, H2;
+    eauto.
++ intros. unfold isConf, isVal, isComp in *. 
+  destruct IHe1 with (V0:=V) (e0 := e1); auto.
+  destruct IHe2  with (V0:=S V) (e0 := e2); auto.
+  destruct H0, H2.
+  repeat split; intros.
+  1: unfold getval; unfold getval in H5.
+  3: unfold getcomp; unfold getcomp in H5. 
+  all:  destruct H5; cbn in H5;
+    destruct getconf eqn:Heq1 in H5; try discriminate;
+    destruct getconf eqn:Heq2 in H5; try discriminate;
+    cbn; destruct H0; eauto; destruct H2; eauto;
+    cbn in H0, H2; rewrite H0, H2;
+    eauto.
++ intros. unfold isConf, isVal, isComp in *. 
+  destruct IHe1 with (V0:=V) (e0 := e1); auto.
+  destruct IHe2  with (V0:=S V) (e0 := e2); auto.
+  destruct H0, H2.
+  repeat split; intros.
+  1: unfold getval; unfold getval in H5.
+  3: unfold getcomp; unfold getcomp in H5. 
+  all:  destruct H5; cbn in H5;
+    destruct getconf eqn:Heq1 in H5; try discriminate;
+    destruct getconf eqn:Heq2 in H5; try discriminate;
+    cbn; destruct H0; eauto; destruct H2; eauto;
+    cbn in H0, H2; rewrite H0, H2;
+    eauto.
++ intros. unfold isConf, isVal, isComp in *. 
+  destruct IHe1 with (V0:=V) (e0 := e1); auto.
+  destruct IHe2  with (V0:=V) (e0 := e2); auto.
+  destruct IHe3  with (V0:=V) (e0 := e3); auto.
+  destruct H0, H2, H4.
+  repeat split; intros.
+  1: unfold getval in H8.
+  3: unfold getcomp in H8.
+  all:
+    cbn in H8; destruct H8; 
+    destruct getconf eqn:? in H8; try discriminate.
+    destruct c eqn:? in H8; try discriminate;
+    destruct e eqn:? in H8; try discriminate;
+    subst;
+    destruct getconf eqn:? in H8; try discriminate;
+    destruct c eqn:? in H8; try discriminate;
+    destruct e eqn:? in H8; try discriminate;
+    subst;
+    destruct getconf eqn:? in H8; try discriminate.
+  1: unfold getval. 
+  3: unfold getcomp.
+  all:
+    cbn;
+    unfold getval in H; destruct H; try rewrite Heqo; eauto;
+    destruct getconf eqn:? in H ; try discriminate;
+    destruct c0 eqn:? in H ; try discriminate;
+    destruct e eqn:? in H ; try discriminate;
+    subst; cbn in Heqo2; rewrite Heqo2;
+
+    unfold getval in H1; destruct H1; try rewrite Heqo0; eauto;
+    destruct getconf eqn:? in H1; try discriminate;
+    destruct c0 eqn:? in H1; try discriminate;
+    destruct e eqn:? in H1; try discriminate;
+    subst; cbn in Heqo3; rewrite Heqo3;
+
+    destruct H4; eauto; cbn in H4; rewrite H4; eauto.
++ repeat split; intros; cbn; (unfold isVal || unfold isConf || unfold isComp); cbn; eauto.
++ repeat split; intros; cbn; (unfold isVal || unfold isConf || unfold isComp); cbn; eauto.
++ repeat split; intros; cbn; (unfold isVal || unfold isConf || unfold isComp); cbn; eauto.
++ repeat split; intros; 
+  destruct IHe1 with (V0:=V) (e0 := e1); auto;
+  destruct IHe2  with (V0:=S V) (e0 := e2); auto;
+  destruct H1, H3;
+  unfold isConf, isVal, isComp in *. 
+  - unfold isVal; unfold getval; cbn. 
+    destruct H. unfold getval in H. cbn in H.
+    destruct getconf eqn:? in H; try discriminate.
+    destruct e eqn:? in H; try discriminate.
+    destruct getconf eqn:? in H; try discriminate.
+  - cbn. 
+    destruct H. cbn in H.
+    destruct getconf eqn:? in H; try discriminate.
+    destruct e eqn:? in H; try discriminate.
+    subst.
+    destruct getconf eqn:? in H; try discriminate.
+   
+    unfold getcomp in H4. rewrite Heqo in H4. 
+    destruct H4; eauto. 
+    destruct getconf eqn:? in H4; try discriminate.
+    destruct e3 eqn:? in H4; try discriminate. subst.
+    cbn in Heqo1. rewrite Heqo1.
+
+    rewrite Heqo0 in H3. destruct H3; eauto.
+    cbn in H3. rewrite H3. eauto.
+  - unfold isComp; unfold getcomp; cbn. 
+    destruct H. unfold getcomp in H. cbn in H.
+    destruct getconf eqn:? in H; try discriminate.
+    destruct e eqn:? in H; try discriminate.
+    destruct getconf eqn:? in H; try discriminate.
++ repeat split; intros; 
+  destruct IHe1 with (V0:=V) (e0 := e1); auto;
+  destruct IHe2  with (V0:= V) (e0 := e2); auto;
+  destruct IHe3 with (V0:= V) (e0 := e3); auto;
+  destruct H1, H3, H5;
+    unfold isConf, isVal, isComp in *. 
+  1: unfold getval; unfold getval in H.
+  3: unfold getcomp; unfold getcomp in H.
+  all: cbn.
+  all:  destruct H; unfold getval in H; cbn in H;
+    destruct getconf eqn:? in H; try discriminate;
+    destruct getconf eqn:? in H; try discriminate;
+    destruct getconf eqn:? in H; try discriminate;
+    destruct e4 eqn:? in H; try discriminate;
+    destruct e5 eqn:? in H; try discriminate.
+  - subst.
+    rewrite Heqo in H3. destruct H3; eauto.
+    cbn in H3. rewrite H3.
+    rewrite Heqo0 in H5. destruct H5; eauto.
+    cbn in H5. rewrite H5.
+    unfold getval in H0. rewrite Heqo1 in H0. destruct H0; eauto.
+    destruct getconf eqn:? in H0; try discriminate. 
+    destruct e4 eqn:? in H0; try discriminate.
+    destruct e5 eqn:? in H0; try discriminate.
+    subst.
+    cbn in Heqo2. rewrite Heqo2. eauto.
++ repeat split; intros;
+  destruct IHe1 with (V0:=V) (e0 := e1); auto;
+  destruct IHe2  with (V0:=V) (e0 := e2); auto;
+  destruct H1, H3;
+  unfold isConf, isVal, isComp in *.
+  3: unfold getcomp in H; unfold getcomp.
+  1: unfold getval in H.
+  all: destruct H; cbn in H;
+    destruct getconf eqn:? in H; try discriminate;
+    destruct e eqn:? in H; try discriminate;
+    destruct e0 eqn:? in H; try discriminate;
+    subst;
+    destruct getconf eqn:? in H; try discriminate;
+    destruct e eqn:? in H; try discriminate;
+    destruct e0 eqn:? in H; try discriminate.
+  all:
+    subst; cbn;
+    unfold getval in H0; rewrite Heqo in H0;  destruct H0; eauto; 
+    destruct getconf eqn:? in H0; try discriminate; 
+    destruct e eqn:? in H0; try discriminate;
+    destruct e0 eqn:? in H0; try discriminate; subst;
+    cbn in Heqo1; rewrite Heqo1;
+    unfold getval in H2; rewrite Heqo0 in H2;  destruct H2; eauto; 
+    destruct getconf eqn:? in H2; try discriminate; 
+    destruct e eqn:? in H2; try discriminate;
+    destruct e0 eqn:? in H2; try discriminate; subst;
+    cbn in Heqo2; rewrite Heqo2; eauto.
++ repeat split; intros; 
+  destruct IHe with (V0:=V) (e0 := e); auto;
+  destruct H1;
+  unfold isConf, isVal, isComp in *.
+  1: unfold getval in H; unfold getval.
+  3: unfold getcomp in H; unfold getcomp.
+  all: cbn in H; destruct H; 
+    destruct getconf eqn:? in H; try discriminate;
+    destruct e0 eqn:? in H; try discriminate;
+    destruct e1 eqn:? in H; try discriminate.
+  all: subst; cbn; unfold getval in H0; rewrite Heqo in H0; destruct H0; eauto;
+    destruct getconf eqn:? in H0; try discriminate;
+    destruct e0 eqn:? in H0; try discriminate;
+    destruct e1 eqn:? in H0; try discriminate;
+    subst; cbn in Heqo0; rewrite Heqo0; eauto.
++ repeat split; intros; destruct IHe with (V0:=V) (e0 := e); auto;
+  destruct H1;
+  unfold isConf, isVal, isComp in *.
+  1: unfold getval in H; unfold getval.
+  3: unfold getcomp in H; unfold getcomp.
+  all: cbn in H; destruct H; 
+    destruct getconf eqn:? in H; try discriminate;
+    destruct e0 eqn:? in H; try discriminate;
+    destruct e1 eqn:? in H; try discriminate.
+  all: subst; cbn; unfold getval in H0; rewrite Heqo in H0; destruct H0; eauto;
+    destruct getconf eqn:? in H0; try discriminate;
+    destruct e0 eqn:? in H0; try discriminate;
+    destruct e1 eqn:? in H0; try discriminate;
+    subst; cbn in Heqo0; rewrite Heqo0; eauto.
+Defined.
+
+Corollary open_preserves_conf {V: nat} (x: name): 
+forall (e: @exp (S V)), (isConf e -> isConf (open x e)).
+Proof. apply open_preserves_ANF. Defined.
+
+Corollary open_preserves_val {V: nat} (x: name): 
+forall (e: @exp (S V)), (isVal e -> isVal (open x e)).
+Proof. apply open_preserves_ANF. Defined.
+
+Corollary open_preserves_comp {V: nat} (x: name): 
+forall (e: @exp (S V)), (isComp e -> isComp (open x e)).
+Proof. apply open_preserves_ANF. Defined.
+
+Definition open_val {V: nat}(x: name)(e: @val (S V)) :=
+(unoption_ex (getval (open x (flattenval (e))))) ((open_preserves_val x (flattenval e)) (flatten_val_is_ANF e)).
+Definition open_comp {V: nat}(x: name)(e: @comp (S V)):=
+(unoption_ex (getcomp (open x (flattencomp (e))))) ((open_preserves_comp x (flattencomp e)) (flatten_comp_is_ANF e)).
+Definition open_conf {V: nat}(x: name)(e: @conf (S V)):=
+(unoption_ex (getconf (open x (flattenconf (e))))) ((open_preserves_conf x (flattenconf e)) (flatten_conf_is_ANF e)).
