ECCA/equiv.v
@@ -1,0 +1,110 @@
+Require Export reduction.
+
+Reserved Notation "g '|-' A '=e=' B"  (at level 250, A at level 99).
+Inductive Equiv: env -> exp -> exp -> Prop :=
+  | aE_RedCong (g: env) (e e1 e2: exp) :
+      RedClos g e1 e ->
+      RedClos g e2 e ->
+      Equiv g e1 e2
+   | aE_RedCongIta1 (g: env) (e1 A e e2 e2': exp) (x: name) :
+      RedClos g e1 (eAbs A e) ->
+      RedClos g e2 e2' ->
+(*       conf_to_val e2' = Some v2' -> *)
+      Equiv (ctx_cons g x (Assum A)) (open x e) (eApp e2' (eId (free x))) ->
+      Equiv g e1 e2 
+   | aE_RedCongIta2 (g: env) (e e1 e1' e2 A : exp) (x: name) :
+      RedClos g e1 e1' ->
+      RedClos g e2 (eAbs A e) ->
+(*       conf_to_val e1' = Some v1' -> *)
+      Equiv (ctx_cons g x (Assum A)) (open x e) (eApp e1' (eId (free x))) -> (* changed order here *)
+      Equiv g e1 e2
+   | aE_Reflect (g : env) (x : atom) (e1 e2 : exp):
+       (has g x (Eq e1 e2)) \/ (has g x (Eq e2 e1)) ->
+       Equiv g e1 e2
+(*   | aE_RedCongAlpha (g: env) (e1 e2: exp):
+      ECCA_Aeq e1 e2 ->
+      Equiv g e1 e2 *)
+(*   | aE_Subst1 (g: env) (e e1 e2 v: exp) (e': exp):
+(*       conf_to_val e = Some v -> *)
+      Equiv g e e' ->
+      Equiv g (eSubst e1 e2 v) e'
+  | aE_Subst2 (g: env) (e1 e2 v: exp) (e e': exp):
+(*       conf_to_val e = Some v -> *)
+      Equiv g e e' ->
+      Equiv g e' (eSubst e1 e2 v) *)
+where "g '|-' A '=e=' B"  := (Equiv g A B): ECCA_scope.
+(*TODO: rewrite with notation for legibility*)
+Bind Scope ECCA_scope with Equiv.
+Hint Constructors Equiv.
+
+(* 
+Reserved Notation "A '=a=' B"  (at level 50).
+Inductive ECCA_Aeq : exp -> exp -> Prop :=
+  | aeq_id (e: exp):
+    e =a= e
+  | aeq_var (x: atom):
+     (eId x) =a= (eId x)
+  | aeq_abs_same (x: atom) (t1 t2 b1 b2: exp):
+     t1 =a= t2 -> 
+     b1 =a= b2 ->
+     (eAbs x t1 b1) =a= (eAbs x t2 b2)
+  | aeq_abs_diff (x y: atom) (t1 t2 b1 b2: exp):
+(*      x <> y -> *)
+     x `notin` (FV b2) ->
+     b1 =a= (swap y x b2) ->
+     t1 =a= t2 ->
+     (eAbs x t1 b1) =a= (eAbs y t2 b2)
+  | aeq_pi_same (x: atom) (t1 t2 b1 b2: exp):
+     t1 =a= t2 -> 
+     b1 =a= b2 ->
+     (ePi x t1 b1) =a= (ePi x t2 b2)
+  | aeq_pi_diff (x y: atom) (t1 t2 b1 b2: exp):
+(*      x <> y ->  Don't think we need this. If x binds nothing, then our new var could be x.*)
+     x `notin` (FV b2) ->
+     b1 =a= (swap y x b2) ->
+     t1 =a= t2 ->
+     (ePi x t1 b1) =a= (ePi y t2 b2)
+  | aeq_let_same (x: atom) (t1 t2 b1 b2: exp):
+     t1 =a= t2 -> 
+     b1 =a= b2 ->
+     (eLet x t1 b1) =a= (eLet x t2 b2)
+  | aeq_let_diff (x y: atom) (t1 t2 b1 b2: exp):
+(*      x <> y -> *)
+     x `notin` (FV b2) ->
+     b1 =a= (swap y x b2) ->
+     t1 =a= t2 ->
+     (eLet x t1 b1) =a= (eLet y t2 b2)
+  | aeq_sig_same (x: atom) (t1 t2 b1 b2: exp):
+     t1 =a= t2 -> 
+     b1 =a= b2 ->
+     (eSig x t1 b1) =a= (eSig x t2 b2)
+  | aeq_sig_diff (x y: atom) (t1 t2 b1 b2: exp):
+(*      x <> y -> *)
+     x `notin` (FV b2) ->
+     b1 =a= (swap y x b2) ->
+     t1 =a= t2 ->
+     (eSig x t1 b1) =a= (eSig y t2 b2)
+  | aeq_app (t1 t2 t1' t2': exp):
+     t1 =a= t1' ->
+     t2 =a= t2' ->
+     (eApp t1 t2) =a= (eApp t1' t2')
+  | aeq_pair (t1 t2 t1' t2' A A': exp):
+     t1 =a= t1' ->
+     t2 =a= t2' ->
+     A  =a= A' ->
+     (ePair t1 t2 A) =a= (ePair t1' t2' A')
+  | aeq_Fst (e e': exp):
+     e =a= e' ->
+     (eFst e) =a= (eFst e')
+  | aeq_Snd (e e': exp):
+     e =a= e' ->
+     (eSnd e) =a= (eSnd e')
+(*   | aeq_if (e1 e2 e3 e1' e2' e3': exp):
+     ECCA_Aeq e1 e1' ->
+     ECCA_Aeq e2 e2' ->
+     ECCA_Aeq e3 e3' ->
+     ECCA_Aeq (eIf e1 e2 e3) (eIf e1' e2' e3')*)
+where "A '=a=' B"  := (ECCA_Aeq A B): ECCA_scope.
+Bind Scope ECCA_scope with ECCA_Aeq.
+Hint Constructors ECCA_Aeq.
+ *)
