ECCA/equiv_lemmas.v
@@ -1,33 +1,33 @@
-Require Export ECCA_equiv.
-Require Import ECCA_reduction_lemmas.
+Require Export equiv.
+Require Import reduction_lemmas.
 Require Import Equivalence.
 
-Lemma equiv_refl (g: ECCAenv): Reflexive (ECCA_Equiv g).
+Lemma equiv_refl (g: env): Reflexive (Equiv g).
 Proof.
 unfold Reflexive. intros.
-apply aE_Equiv with (e:= x); auto.
+apply aE_RedCong with (e:= x); auto.
 Qed.
 
-Lemma equiv_sym (g: ECCAenv): Symmetric (ECCA_Equiv g).
+Lemma equiv_sym (g: env): Symmetric (Equiv g).
 Proof.
 unfold Symmetric. intros. inversion H.
-- apply aE_Equiv with (e := e); auto.
-- subst. apply aE_EquivIta2 with (x:=x0) (e2:=x) (e1':=e2')(e1:=y)(A:= A)(e:=e).
+- apply aE_RedCong with (e := e); auto.
+- subst. apply aE_RedCongIta2 with (x:=x0) (e2:=x) (e1':=e2')(e1:=y)(A:= A)(e:=e).
   + auto.
   + apply H0.
   + apply H2. 
-- subst. eapply aE_EquivIta1.
+- subst. eapply aE_RedCongIta1.
   + apply H1.
   + apply H0.
   + apply H2.
 - subst. eapply aE_Reflect. apply or_comm. apply H0.
 Qed.
 
-Lemma equiv_trans (g: ECCAenv): Transitive (ECCA_Equiv g).
+Lemma equiv_trans (g: env): Transitive (Equiv g).
 Proof.
 unfold Transitive. intros. induction H; induction H0; subst.
 - cut (exists d, (g |- e =r> d) /\ (g |- e0 =r> d))%ECCA.
-  + intros. destruct H3. destruct H3. apply aE_Equiv with (e:=x).
+  + intros. destruct H3. destruct H3. apply aE_RedCong with (e:=x).
     * apply R_Trans with (e':=e); auto.
     * apply R_Trans with (e':=e0); auto.
   + apply church_rosser with (e:=e2); auto.
@@ -36,16 +36,16 @@ unfold Transitive. intros. induction H; induction H0; subst.
 (*need more church rosser stuff for the eta-equivalence cases.*)
 Admitted.
 
-Lemma equiv_weakening (g: ECCAenv) (x: name) (a: ctxmem) (e1 e2: ECCAexp):
-  (ECCA_Equiv g e1 e2) ->
-  (ECCA_Equiv (ctx_cons g x a) e1 e2).
+Lemma equiv_weakening (g: env) (x: name) (a: ctxmem) (e1 e2: exp):
+  (Equiv g e1 e2) ->
+  (Equiv (ctx_cons g x a) e1 e2).
 Admitted.
 
-Lemma if_cong_v_equiv (g: ECCAenv) (v v' m1 m2: ECCAexp):
-  (ECCA_Equiv g v v') ->
-  (ECCA_Equiv g (eIf v m1 m2) (eIf v' m1 m2)).
+Lemma if_cong_v_equiv (g: env) (v v' m1 m2: exp):
+  (Equiv g v v') ->
+  (Equiv g (eIf v m1 m2) (eIf v' m1 m2)).
 Proof.
-  intros. inversion H. 1,2,3: eapply aE_Equiv.
+  intros. inversion H. 1,2,3: eapply aE_RedCong.
   - apply R_CongIf. apply H0. apply R_Refl. apply R_Refl.
   - apply R_CongIf. apply H1. apply R_Refl. apply R_Refl.
   - apply R_CongIf. apply H0. apply R_Refl. apply R_Refl.
@@ -55,62 +55,62 @@ Proof.
   - admit.
 Admitted.
 
-Lemma if_eta_1 (g: ECCAenv) (x: name) (v m1 m2 m: ECCAexp):
-  (ECCA_Equiv g (eIf v m1 m2) m) ->
-  (ECCA_Equiv (ctx_cons g x (Eq v eTru)) m1 m).
+Lemma if_eta_1 (g: env) (x: name) (v m1 m2 m: exp):
+  (Equiv g (eIf v m1 m2) m) ->
+  (Equiv (ctx_cons g x (Eq v eTru)) m1 m).
 Proof.
   intros.
-  cut (ECCA_Equiv (ctx_cons g x (Eq v eTru)) (eIf v m1 m2) (eIf eTru m1 m2)).
+  cut (Equiv (ctx_cons g x (Eq v eTru)) (eIf v m1 m2) (eIf eTru m1 m2)).
   - intros.
-    cut (ECCA_Equiv (ctx_cons g x (Eq v eTru)) (eIf eTru m1 m2) m1).
+    cut (Equiv (ctx_cons g x (Eq v eTru)) (eIf eTru m1 m2) m1).
     + intros. apply equiv_weakening with (x:=x) (a:=Eq v eTru) in H.
       eapply equiv_trans. apply equiv_sym in H1. apply H1.
       eapply equiv_trans. apply equiv_sym in H0. apply H0.
       assumption.
-    + apply aE_Equiv with (e:=m1).
+    + apply aE_RedCong with (e:=m1).
       * apply R_RedR. auto.
       * apply R_Refl.
-  - cut (ECCA_Equiv (ctx_cons g x (Eq v eTru)) v eTru).
+  - cut (Equiv (ctx_cons g x (Eq v eTru)) v eTru).
     + intros. apply if_cong_v_equiv. assumption.
     + apply aE_Reflect with (x:=(free x)). left. apply ctx_has.
 Qed.
 
-Lemma if_eta_2 (g: ECCAenv) (x: name) (v m1 m2 m: ECCAexp):
-  (ECCA_Equiv g (eIf v m1 m2) m) ->
-  (ECCA_Equiv (ctx_cons g x (Eq v eFls)) m2 m).
+Lemma if_eta_2 (g: env) (x: name) (v m1 m2 m: exp):
+  (Equiv g (eIf v m1 m2) m) ->
+  (Equiv (ctx_cons g x (Eq v eFls)) m2 m).
 Proof.
   intros.
-  cut (ECCA_Equiv (ctx_cons g x (Eq v eFls)) (eIf v m1 m2) (eIf eFls m1 m2)).
+  cut (Equiv (ctx_cons g x (Eq v eFls)) (eIf v m1 m2) (eIf eFls m1 m2)).
   - intros.
-    cut (ECCA_Equiv (ctx_cons g x (Eq v eFls)) (eIf eFls m1 m2) m2).
+    cut (Equiv (ctx_cons g x (Eq v eFls)) (eIf eFls m1 m2) m2).
     + intros. apply equiv_weakening with (x:=x) (a:=Eq v eFls) in H.
       eapply equiv_trans. apply equiv_sym in H1. apply H1.
       eapply equiv_trans. apply equiv_sym in H0. apply H0.
       assumption.
-    + apply aE_Equiv with (e:=m2).
+    + apply aE_RedCong with (e:=m2).
       * apply R_RedR. auto.
       * apply R_Refl.
-  - cut (ECCA_Equiv (ctx_cons g x (Eq v eFls)) v eFls).
+  - cut (Equiv (ctx_cons g x (Eq v eFls)) v eFls).
     + intros. apply if_cong_v_equiv. assumption.
     + apply aE_Reflect with (x:=(free x)). left. apply ctx_has.
 Qed.
 
-Instance ECCA_Equiv_equiv (g: ECCAenv) : Equivalence (ECCA_Equiv g).
+Instance Equiv_equiv (g: env) : Equivalence (Equiv g).
 Proof.
 split. apply equiv_refl. apply equiv_sym. apply equiv_trans.
 Qed.
-Hint Resolve ECCA_Equiv_equiv.
+Hint Resolve Equiv_equiv.
 Require Import String.
 
-(*TODO: To use this, we need to declare some functions proper wrt to ECCA_equiv.
+(*TODO: To use this, we need to declare some functions proper wrt to equiv.
 Then we can do rewriting. 
 See page 17 of 
 https://www.labri.fr/perso/casteran/CoqArt/TypeClassesTut/typeclassestut.pdf *)
 
-(* Require Import ECCA_typing. *)
+(* Require Import typing. *)
 
 (* 
-Lemma equiv_distributes_over_pi (g: ECCAenv) (x: atom) (B B' A A': ECCAexp):
+Lemma equiv_distributes_over_pi (g: env) (x: atom) (B B' A A': exp):
 (g |- A =e= A' ->
 g |- B =e= B' ->
 g |- ePi x A B =e= ePi x A' B')%ECCA.
@@ -118,7 +118,7 @@ Proof.
 intros. inversion H. inversion H0.
 - subst.
 
-Lemma equiv_equivariant_over_subst (g: ECCAenv) (x: atom) (N N' A B: ECCAexp):
+Lemma equiv_equivariant_over_subst (g: env) (x: atom) (N N' A B: exp):
 (g |- N : A ->
 g |- N' : A ->
 g |- N =e= N' ->
@@ -129,7 +129,7 @@ intros. induction H1.
 - rewrite substWork_equation. rewrite substWork_equation.
  destruct AtomSetImpl.mem.
   + induction B; auto. destruct (x == x0); auto.
-    * eapply aE_Equiv with (e := e); auto.
+    * eapply aE_RedCong with (e := e); auto.
     * destruct (x == x0).
       ++
 
@@ -145,26 +145,26 @@ intros. induction H1.
 
    
 - *)
-(* Lemma equiv_abs_compositional_1 (g: ECCAenv) (A A' b: ECCAexp): 
-(ECCA_Equiv g A A') ->
-(ECCA_Equiv g (eAbs A b) (eAbs A' b))%ECCA.
+(* Lemma equiv_abs_compositional_1 (g: env) (A A' b: exp): 
+(Equiv g A A') ->
+(Equiv g (eAbs A b) (eAbs A' b))%ECCA.
 Proof.
 intros. inversion H.
-+ subst. apply aE_Equiv with (e:=eAbs e b); eapply R_CongLam1; auto.
++ subst. apply aE_RedCong with (e:=eAbs e b); eapply R_CongLam1; auto.
 Admitted.
 
-Lemma equiv_abs_compositional_2 (g: ECCAenv) (x: atom) (A b b': ECCAexp): 
-(ECCA_Equiv (Assum g x A) b b') ->
-(ECCA_Equiv g (eAbs x A b) (eAbs x A b'))%ECCA.
+Lemma equiv_abs_compositional_2 (g: env) (x: atom) (A b b': exp): 
+(Equiv (Assum g x A) b b') ->
+(Equiv g (eAbs x A b) (eAbs x A b'))%ECCA.
 Proof.
 intros. induction H.
-+ apply aE_Equiv with (e:=eAbs x A e); apply R_CongLam1; auto.
++ apply aE_RedCong with (e:=eAbs x A e); apply R_CongLam1; auto.
 Admitted.
 
-Lemma equiv_abs_compositional (g: ECCAenv) (x: atom) (A A' b b': ECCAexp): 
-(ECCA_Equiv g A A') ->
-(ECCA_Equiv (Assum g x A) b b') ->
-(ECCA_Equiv g (eAbs x A b) (eAbs x A' b'))%ECCA.
+Lemma equiv_abs_compositional (g: env) (x: atom) (A A' b b': exp): 
+(Equiv g A A') ->
+(Equiv (Assum g x A) b b') ->
+(Equiv g (eAbs x A b) (eAbs x A' b'))%ECCA.
 Proof.
 intros.
 Admitted.
