ECCA/key_lemmas.v
@@ -1,0 +1,93 @@
+Require Export typing.
+Require Export equiv_lemmas.
+Require Export continuations.
+Require Export ECCA_het_comp.
+
+Lemma Cut (g: env) (K : cont) (N: exp) (A B: exp):
+(Types_cont g K (Cont N A B) ->
+Types g N A ->
+Types g (fill_hole N K) B)%ECCA.
+Proof. 
+intros. inversion H ; subst ; cbv.
+- assumption. 
+- cut (@bind N 0 (@wk 0 B) = B); simpl_term_eq. 
+  intros. rewrite <- H1. eapply aT_Let with (n:= N) (m:= M) (A:=A) (B:=(wk B)) (x:=y) (g:=g); assumption.
+Qed.
+
+Lemma weakening (g : env) (x : name) (N A A' : exp):
+  Types g N A ->
+  Types (ctx_cons g x (Assum A')) N A.
+Proof.
+Admitted.
+
+Lemma def_weakening (g : env) (x : name) (N N' A A' : exp):
+  Types g N A ->
+  Types (ctx_cons g x (Def N' A')) N A.
+Admitted.
+
+Lemma append_env_weakening (g g': env) (N A : exp):
+  Types g N A ->
+  Types (append g g') N A.
+Proof.
+Admitted.
+
+Lemma append_env_equiv_weakening (g g': env) (e e' : exp):
+  Equiv g e e' ->
+  Equiv (append g g') e e'.
+Proof.
+Admitted.
+
+Lemma equivalence_in_derivation (g: env) (N N' M : exp) (A B : exp) (x : name):
+Types g N A ->
+Types g N' A ->
+Equiv g N N' ->
+Types (ctx_cons g x (Def N A)) M B ->
+Types (ctx_cons g x (Def N' A)) M B.
+Admitted.
+
+  
+Lemma Cut_modulo_equivalence (g: env) (K : cont) (N N': exp) (A B: exp):
+(Types_cont g K (Cont N A B) ->
+Types g N A ->
+Types g N' A ->
+Equiv g N N' ->
+Types g (fill_hole N' K) B)%ECCA.
+Proof. 
+intros. inversion H ; subst ; cbv.
+- assumption. 
+- cut (@bind N' 0 (@wk 0 B) = B); simpl_term_eq.
+  intros. rewrite <- H3. eapply aT_Let with (n:= N') (m:= M) (A:=A) (B:=(wk B)) (x:=y) (g:=g).
+  * assumption.
+  * apply equivalence_in_derivation with (N := N); assumption.
+Qed. 
+
+Lemma het_compose_equal_fill_hole (K : cont_r) (N: comp) :
+  (flattenconf (het_compose_r K (Comp N))) = (fill_hole N (@unrestrict_cont 0 K)).
+Proof.
+  destruct K; simpl; auto.
+Qed.  
+
+Lemma append_rearrange {V:nat}(g g': @env V) (x: name) (a: ctxmem) :
+  ((append g g')& x ~ a) = (append (g & x ~ a) g').
+Proof.
+  induction g; simpl; auto.
+Qed.
+
+Lemma Hetereogeneous_Cut (g g': env) (K : cont_r) (M M': conf) (A B: exp):
+Types_cont (append g g') (unrestrict_cont K) (Cont M' A B) ->
+Types g M A ->
+(@WellBound_conf 0 g M) ->
+Equiv g M M' ->
+Types (append g g') (het_compose_r K M) B.
+Proof.
+  intros. induction H1.
+  - erewrite het_compose_equal_fill_hole. apply Cut_modulo_equivalence with (A := A) (N:=M').
+    assumption. inversion H. assumption. assumption. apply append_env_weakening with (g':=g') in H0.
+    assumption. apply equiv_sym. apply append_env_equiv_weakening with (g':=g') in H2. assumption.
+  - simpl. inversion H. inversion H0. rewrite <- H8. rewrite <- H13. apply aT_Let with (A:=A2) (x:=x0).
+    + apply append_env_weakening with (g':=g') in H12. assumption.
+    + erewrite append_rearrange. admit.
+      
+Admitted.
+
+ 
